src/Andrea_proof.thy
@@ -20,12 +20,32 @@ lemma fst_snd_simps: "((a,b)|>fst = a) & ((a,b)|>snd = b)"
 apply(simp add:rev_apply_def)
 done
   
-
 lemma wellformed_context_hereditary: "wellformed_context (x#xs) \<Longrightarrow> wellformed_context xs"
 apply (case_tac xs)
  apply (force simp add:wellformed_context_def)+
 done
 
+lemma wellformed_context_i_less_than_length_rs:
+"wellformed_context (((ks, rs), i) # stk) \<Longrightarrow> i \<le> length ks \<and> i < length rs"
+apply (induct stk)
+ apply (simp add:wellformed_context_def)
+ apply (simp add:wellformed_tree_def wf_ks_rs_def forall_subtrees_def rev_apply_def wf_ks_rs_1_def)
+
+ apply (simp add:wellformed_context_def)
+ apply (case_tac "stk =[]")
+  (*stk = []*)
+  apply (case_tac a, case_tac aa)
+  apply (simp add:wellformed_context_1_def)
+  apply (simp add:wellformed_tree_def wf_ks_rs_def forall_subtrees_def rev_apply_def wf_ks_rs_1_def)
+
+  (*stk = aa#list*)
+  apply simp
+  apply (case_tac "last stk")
+  apply simp
+  apply (case_tac aa)
+  apply (simp add:wellformed_context_1_def)
+done
+  
 lemma list_all_update: "list_all P l \<Longrightarrow> P a \<Longrightarrow> list_all P (l[i := a]) "
 by (metis length_list_update list_all_length nth_list_update_eq nth_list_update_neq) 
 
@@ -34,27 +54,49 @@ lemma list_all_update_concat_map_subtrees:
 list_all P (concat (map tree_to_subtrees (rs[i := t])))"
 by (smt concat.simps(2) concat_append id_take_nth_drop list.map(2) list_all_append list_update_beyond map_append not_le upd_conv_take_nth_drop)
 
+lemma list_all_take_drop_less_one_element: 
+"list_all P xs \<Longrightarrow> (list_all P (take (i- Suc 0) xs)) \<and> (list_all P (drop i xs))"
+by (metis append_take_drop_id list_all_append)
 
-lemma list_all_concat_map_tree_subtrees:
-"(list_all P (concat (map tree_to_subtrees rs))) =               
- (list_all P rs \<and> list_all P (concat (map (\<lambda> t. case t of Node(l,cs) \<Rightarrow> (List.map tree_to_subtrees cs) |> List.concat | Leaf _ \<Rightarrow> []) rs)))"
-apply (induct rs)
- apply simp
+lemma list_all_of_list_replace_at_n:
+"i < length rs \<Longrightarrow>
+ list_replace_at_n ((ks, rs) |> snd) i [tleft, tright] |> dest_Some = rs2 \<Longrightarrow>
+ P tleft \<Longrightarrow>
+ P tright \<Longrightarrow>
+ list_all P rs \<Longrightarrow> list_all P rs2"
+apply (simp_all add:list_replace_at_n_def rev_apply_def split_at_def)
+apply (drule_tac t="rs2" in sym)
+ apply (case_tac "i=0")
+ (*i=0*)
+ apply (case_tac rs,simp+)
 
- apply (case_tac a)
-  apply simp
-  apply (case_tac x1)
-   apply force
-
-  apply force
+ (*i\<noteq>0*)
+ apply (simp add:butlast_take list_all_take_drop_less_one_element)
 done
 
-lemma wf_size_hereditary: "wf_size (Rmbs b) (Node(ks,x#xs)) \<Longrightarrow> wf_size (Rmbs b) (Node (ks,xs))"
-apply (simp add:wf_size_def)
-apply (case_tac b)
-  apply simp
 
-  apply (simp add:forall_subtrees_def rev_apply_def wf_size_1_def)
+lemma list_all_take_drop_less_one_element_concat_map_subtrees:
+"list_all P (concat (map tree_to_subtrees xs)) \<Longrightarrow> 
+(list_all P (concat (map tree_to_subtrees (take (i- Suc 0) xs)))) 
+\<and> (list_all P (concat (map tree_to_subtrees (drop i  xs))))"
+by (metis append_take_drop_id concat_append list_all_append map_append)
+
+lemma list_all_of_list_replace_at_n_concat_map_subtrees:
+"
+i < length rs \<Longrightarrow>
+dest_Some (list_replace_at_n rs i [tleft, tright]) = rs2 \<Longrightarrow>
+list_all P (concat (map tree_to_subtrees rs)) \<Longrightarrow>
+list_all P (tree_to_subtrees tleft) \<Longrightarrow>
+list_all P (tree_to_subtrees tright) \<Longrightarrow>
+list_all P (concat (map tree_to_subtrees rs2))
+"
+apply (simp_all add:list_replace_at_n_def rev_apply_def split_at_def)
+apply (drule_tac t="rs2" in sym)
+  (*i=0*)
+ apply (case_tac rs,simp+)
+
+ (*i\<noteq>0*)
+ apply (simp add:butlast_take list_all_take_drop_less_one_element_concat_map_subtrees)
 done
 
 lemma invariant_wf_ts: "invariant_wf_ts"
@@ -86,12 +128,8 @@ prefer 2
 apply(intro conjI)
  (* wf_focus *)
  apply(simp add: wellformed_focus_def )
- apply(case_tac f)
-  (* inserting_one *) (*A: this case is easier, because the stepped focus can be only insert_one *)
-  apply(rename_tac t)
-  apply(simp)
-  apply(simp add: update_focus_at_position_def)
-  apply(subgoal_tac "wellformed_tree (Rmbs (stk=[])) (Node (ks,rs))") (* A: given that the tree without update is wf, we just need to check that rs was wf (replacing an element will leave it as before)*)
+ apply (subgoal_tac "i<length rs") prefer 2 apply (force simp add:wellformed_context_i_less_than_length_rs)
+ apply(subgoal_tac "wellformed_tree (Rmbs (stk=[])) (Node (ks,rs))") (* A: given that the tree without update is wf, we just need to check that rs was wf (replacing an element will leave it as before)*)
   prefer 2
    apply(simp add: wellformed_context_def)
    apply (subgoal_tac "\<exists> ks' rs' i'. (if stk = [] then ((ks, rs), i) else last stk) = ((ks', rs'), i')")
@@ -108,34 +146,14 @@ apply(intro conjI)
     apply simp
     apply (elim conjE)
     apply (simp add:wellformed_context_1_def)
-
+ apply(case_tac f)
+  (* inserting_one *) (*A: this case is easier, because the stepped focus can be only insert_one *)
+  apply(rename_tac t)
+  apply(simp)
+  apply(simp add: update_focus_at_position_def)
   apply(simp add: wellformed_tree_def)
   apply(elim conjE)
   apply (simp add:list_replace_1_at_n_def dest_Some_def)
-(*  apply (subgoal_tac "\<exists> x. rs!i = x") prefer 2 apply force
-  apply (erule exE)
-  apply (subgoal_tac "\<exists> rs1 rs2. (rs  = rs1@x#rs2)")
-  prefer 2
-   apply (case_tac "rs = []")
-    apply (force intro:FIXME)
-
-    apply (case_tac "i < length rs")
-     
-     apply (blast intro:id_take_nth_drop)
-
-     apply (force intro:FIXME)
-  apply (elim exE)+
-  apply (subgoal_tac "(rs [i:=t ] = rs1@t#rs2)")
-  prefer 2
-   apply (subgoal_tac "length rs = length (rs1 @ x # rs2)") prefer 2 apply force
-   apply (subgoal_tac "i = length rs1 ")
-   prefer 2
-    apply meson
-    apply (subgoal_tac "(length rs) = (length (rs1@(rs!i)#rs2))") prefer 2 apply force
-    apply (force intro:FIXME)
-      
-   apply simp
-*)   
   apply(intro conjI)
    (*wf_size (Rmbs (stk = [])) (Node (ks, rs[i := t]))*)
    apply (simp add:wf_size_def)
@@ -155,18 +173,10 @@ apply(intro conjI)
    (* balanced (Node (ks, rs[i := t])) *)
    apply (case_tac "rs \<noteq> []")
     (* rs \<noteq> [] *)
-    apply (subgoal_tac "i < length rs \<and> (height (rs!i) = height t) ") 
+    apply (subgoal_tac "(height (rs!i) = height t) ") 
     prefer 2
-     apply (intro conjI)
-      (* i < length rs *)
-      apply (simp add:wellformed_context_def)
-      apply (case_tac stk)
-       apply (simp add:wf_ks_rs_def forall_subtrees_def rev_apply_def wf_ks_rs_1_def)
-     
-       apply (force intro:FIXME) (* I need to induct to solve this *)
-
-      (* (height (rs!i) = height t) *)
-      apply (simp add:wellformed_ts_1_def dest_ts_def)
+     (* (height (rs!i) = height t) *)
+     apply (simp add:wellformed_ts_1_def dest_ts_def)
     apply (simp add:balanced_def forall_subtrees_def rev_apply_def balanced_1_def del:height.simps)
     apply (elim conjE)+
     (* now I know that height rs!i = height t, so a substitution should not do any harm*)
@@ -193,8 +203,8 @@ apply(intro conjI)
       \<forall>k\<in>set(keys t). key_le k (ks!i)
       then I can divide the \<forall>ia on the ith index
       *)
-     apply (subgoal_tac "i \<le> length ks") prefer 2 apply (force intro:FIXME)
-     apply (subgoal_tac "length ks  = length rs - 1") prefer 2 apply (force intro:FIXME)
+     apply (subgoal_tac "i \<le> length ks") prefer 2 apply (simp add:wellformed_context_i_less_than_length_rs)
+     apply (subgoal_tac "length ks  = length rs - 1") prefer 2 apply (force simp add:wf_ks_rs_def forall_subtrees_def rev_apply_def wf_ks_rs_1_def)
      apply simp
      apply (case_tac "i \<le> length rs - Suc (Suc 0)")
       apply (subgoal_tac 
@@ -202,19 +212,18 @@ apply(intro conjI)
        ((\<forall>i\<in>{0.. i - 1}. \<forall>k\<in>set (keys (rs ! i)). key_le (ks ! i) k) 
        \<and> ((i \<le> length rs - Suc (Suc 0)) \<longrightarrow> (\<forall>k\<in>set (keys (rs[i := t] ! i)). key_le (ks ! i) k)) 
        \<and> (\<forall>i\<in>{i+1.. length rs - Suc (Suc 0)}. \<forall>k\<in>set (keys (rs ! i)). key_le (ks ! i) k))
-       ") prefer 2 apply simp apply (metis atLeastAtMost_iff le0 nth_list_update_neq)
+       ") prefer 2 apply (thin_tac "i < length rs") apply simp apply (metis atLeastAtMost_iff le0 nth_list_update_neq) 
       apply (subgoal_tac "
         (\<forall>ia\<in>{0..length rs - Suc (Suc 0)}. \<forall>k\<in>set (keys (rs[i := t]!ia)). key_lt k (ks ! (Suc ia))) =
         ((\<forall>i\<in>{0.. i - 1}. \<forall>k\<in>set (keys (rs ! i)). key_lt k (ks ! Suc i)) 
        \<and> ((i \<le> length rs - Suc (Suc 0)) \<longrightarrow> (\<forall>k\<in>set (keys (rs[i := t] ! i)). key_lt k (ks ! Suc i))) 
        \<and> (\<forall>i\<in>{i+1.. length rs - Suc (Suc 0)}. \<forall>k\<in>set (keys (rs ! i)). key_lt k (ks ! Suc i)))
-        ") prefer 2 apply simp apply (metis atLeastAtMost_iff le0 nth_list_update_neq) 
+        ") prefer 2 apply (thin_tac "i < length rs") apply simp apply (metis atLeastAtMost_iff le0 nth_list_update_neq) 
       apply (simp add:wellformed_ts_1_def dest_ts_def check_keys_def)
       apply (case_tac i)
        apply (case_tac rs, force, force)
 
        apply force
-      apply force
 
     (* list_all keys_consistent_1 (concat (map tree_to_subtrees (rs[i := t]))) *)
     apply (subgoal_tac "list_all keys_consistent_1 (tree_to_subtrees t)") prefer 2 apply force
@@ -228,18 +237,70 @@ apply(intro conjI)
   (* inserting_two *)
   apply(simp)
   apply(case_tac x2)
-  apply(rename_tac tleft k0 tr)
+  apply(rename_tac tleft k0 tright)
   apply(simp add: update_focus_at_position_def)
   apply(elim conjE)
   apply(thin_tac "x2 = _")
-  apply(subgoal_tac "? ks2.  list_insert_at_n (n |> fst) i [k0] = ks2") prefer 2 apply(force)
-  apply(subgoal_tac "? rs2. list_replace_at_n (n |> snd) i [tleft, tr] |> dest_Some = rs2") prefer 2 apply(force)
+  apply(subgoal_tac "? ks2. list_insert_at_n (n |> fst) i [k0] = ks2") prefer 2 apply(force)
+  apply(subgoal_tac "? rs2. list_replace_at_n (n |> snd) i [tleft, tright] |> dest_Some = rs2") prefer 2 apply(force)
   apply(elim exE)
   apply(simp add: Let_def)
   apply(case_tac "length ks2 \<le> max_node_keys")
    apply(simp)
-   apply(force intro: FIXME)
+   apply (simp add:wellformed_tree_def)
+   apply(subgoal_tac "length ks2 = Suc (length ks)")
+   prefer 2 apply (force simp add:list_insert_at_n_def rev_apply_def split_at_def)
+   apply (intro conjI)
+    (*wf_size (Rmbs (stk = [])) (Node (ks2, rs2)) *)
+    apply (simp add:wf_size_def)
+    apply (subgoal_tac "wf_size_1 tleft \<and> wf_size_1 tright") prefer 2 apply (force intro:FIXME)
+    apply (elim conjE)+
+    apply (case_tac "stk=[]")
+     (* stk = []*)
+     apply (simp add:list_all_of_list_replace_at_n)
 
+     (* stk \<noteq> [] *)
+     apply (simp add:forall_subtrees_def Let_def rev_apply_def wf_size_1_def)
+     apply (simp add:list_all_of_list_replace_at_n_concat_map_subtrees)
+    
+    (* wf_ks_rs (Node (ks2, take (i - Suc 0) rs @ tleft # tright # drop i rs)) *)
+    apply (simp add:wf_ks_rs_def forall_subtrees_def rev_apply_def )
+    apply (simp add:list_all_of_list_replace_at_n_concat_map_subtrees)  
+    apply (simp add:wf_ks_rs_1_def)
+    apply (simp add:list_replace_at_n_def)
+    apply (simp add:split_at_def)
+    apply (case_tac "i=0",force,force simp add:butlast_take)
+
+    (* balanced (Node (ks2, take (i - Suc 0) rs @ tleft # tright # drop i rs)) *)
+    apply (simp add:balanced_def forall_subtrees_def rev_apply_def)
+    apply (simp add:list_all_of_list_replace_at_n_concat_map_subtrees)  
+    apply (simp add:balanced_1_def del:height.simps)
+    apply (subgoal_tac "list_replace_at_n ((ks, rs) |> snd) i [tleft, tright] |> dest_Some = rs2") prefer 2 apply (force simp add:rev_apply_def)
+    apply (subgoal_tac "height tright = height (rs!0) \<and> height tleft = height (rs!0)") prefer 2 apply (simp add:wellformed_ts_1_def dest_ts_def Let_def del:height.simps) apply (force intro:FIXME)
+    apply (subgoal_tac "height (rs2!0) = height (rs!0)")
+    prefer 2 
+     apply (simp add:list_replace_at_n_def rev_apply_def split_at_def del:height.simps)
+     apply (case_tac "i=0")
+      (* i = 0 *)
+      apply force
+
+      (* i \<noteq> 0 *)
+      apply (simp add:butlast_take del:height.simps)
+      apply (case_tac "take (i - Suc 0) rs")
+       apply force
+
+       apply (metis append_Cons append_take_drop_id nth_Cons_0)
+    apply (case_tac "rs2 = []", simp)
+    apply (force simp add: list_all_of_list_replace_at_n)
+
+    (* keys_consistent (Node (ks2, take (i - Suc 0) rs @ tleft # tright # drop i rs)) *)
+    apply(force intro: FIXME)
+
+    (* keys_ordered (Node (ks2, take (i - Suc 0) rs @ tleft # tright # drop i rs)) *)
+    apply (simp add:keys_ordered_def forall_subtrees_def rev_apply_def)
+    apply (simp add:list_all_of_list_replace_at_n_concat_map_subtrees)
+    apply (simp add:keys_ordered_1_def ordered_key_list_def)
+    apply(force intro: FIXME)
    apply(simp)
    apply(simp add: split_node_def)
    apply(force intro: FIXME)
